Update Comparse

fstar/MLS.NetworkTypes.fst
@@ -126,14 +126,14 @@ val ps_option_length: #bytes:Type0 -> {|bytes_like bytes|} -> #a:Type0 -> ps_a:p
 let ps_option_length #bytes #bl #a ps_a x =
   reveal_opaque (`%ps_option) (ps_option ps_a)
 
-val ps_option_is_valid: #bytes:Type0 -> {|bytes_like bytes|} -> #a:Type0 -> ps_a:parser_serializer bytes a -> pre:bytes_compatible_pre bytes -> x:option a -> Lemma (
-  (ps_option ps_a).is_valid pre x <==> (
+val ps_option_is_well_formed: #bytes:Type0 -> {|bytes_like bytes|} -> #a:Type0 -> ps_a:parser_serializer bytes a -> pre:bytes_compatible_pre bytes -> x:option a -> Lemma (
+  is_well_formed_partial (ps_option ps_a) pre x <==> (
     match x with
     | None -> True
-    | Some y -> ps_a.is_valid pre y
+    | Some y -> is_well_formed_partial ps_a pre y
   ))
-  [SMTPat ((ps_option ps_a).is_valid pre x)]
-let ps_option_is_valid #bytes #bl #a ps_a pre x =
+  [SMTPat (is_well_formed_partial (ps_option ps_a) pre x)]
+let ps_option_is_well_formed #bytes #bl #a ps_a pre x =
   reveal_opaque (`%ps_option) (ps_option ps_a)
 
 /// struct {
