fstar/MLS.Symbolic.Parsers.fst
@@ -20,7 +20,7 @@ noeq type tree_internal_node (bytes:Type0) {|bytes_like bytes|} (leaf_t:Type0) (
 }
 
 %splice [ps_tree_internal_node] (gen_parser (`tree_internal_node))
-%splice [ps_tree_internal_node_is_valid] (gen_is_valid_lemma (`tree_internal_node))
+%splice [ps_tree_internal_node_is_well_formed] (gen_is_well_formed_lemma (`tree_internal_node))
 
 [@@"opaque_to_smt"]
 val ps_tree: #bytes:Type0 -> {|bytes_like bytes|} -> #leaf_t:Type0 -> #node_t:Type0 -> parser_serializer bytes leaf_t -> parser_serializer_unit bytes node_t -> l:nat -> i:tree_index l -> parser_serializer bytes (tree leaf_t node_t l i)
@@ -39,14 +39,14 @@ let rec ps_tree #bytes #bl #leaf_t #node_t ps_leaf_t ps_node_t l i =
       (fun (TNode data left right) -> {left; data; right})
   )
 
-val ps_tree_is_valid: #bytes:Type0 -> {|bytes_like bytes|} -> #leaf_t:Type0 -> #node_t:Type0 -> ps_leaf_t:parser_serializer bytes leaf_t -> ps_node_t:parser_serializer_unit bytes node_t -> l:nat -> i:tree_index l -> pre:bytes_compatible_pre bytes -> x:tree leaf_t node_t l i -> Lemma
-  ((ps_tree ps_leaf_t ps_node_t l i).is_valid pre x <==> (
+val ps_tree_is_well_formed: #bytes:Type0 -> {|bytes_like bytes|} -> #leaf_t:Type0 -> #node_t:Type0 -> ps_leaf_t:parser_serializer bytes leaf_t -> ps_node_t:parser_serializer_unit bytes node_t -> l:nat -> i:tree_index l -> pre:bytes_compatible_pre bytes -> x:tree leaf_t node_t l i -> Lemma
+  (is_well_formed_partial (ps_tree ps_leaf_t ps_node_t l i) pre x <==> (
     match x with
-    | TLeaf y -> ps_leaf_t.is_valid pre y
-    | TNode y left right -> ps_node_t.is_valid pre y /\ (ps_tree ps_leaf_t ps_node_t (l-1) (left_index i)).is_valid pre left /\ (ps_tree ps_leaf_t ps_node_t (l-1) (right_index i)).is_valid pre right
+    | TLeaf y -> is_well_formed_partial ps_leaf_t pre y
+    | TNode y left right -> is_well_formed_partial ps_node_t pre y /\ is_well_formed_partial (ps_tree ps_leaf_t ps_node_t (l-1) (left_index i)) pre left /\ is_well_formed_partial (ps_tree ps_leaf_t ps_node_t (l-1) (right_index i)) pre right
   ))
-  [SMTPat ((ps_tree ps_leaf_t ps_node_t l i).is_valid pre x)]
-let ps_tree_is_valid #bytes #bl #leaf_t #node_t ps_leaf_t ps_node_t l i pre x =
+  [SMTPat (is_well_formed_partial (ps_tree ps_leaf_t ps_node_t l i) pre x)]
+let ps_tree_is_well_formed #bytes #bl #leaf_t #node_t ps_leaf_t ps_node_t l i pre x =
   // For some reason, reveal_opaque doesn't work here
   normalize_term_spec (ps_tree ps_leaf_t ps_node_t l i)
 
@@ -54,14 +54,14 @@ val ps_treesync: #bytes:Type0 -> {|bytes_like bytes|} -> tkt:treekem_types bytes
 let ps_treesync #bytes tkt l i =
   ps_tree (ps_option (ps_leaf_node_nt tkt)) (ps_option (ps_parent_node_nt tkt)) l i
 
-val ps_treesync_is_valid: #bytes:Type0 -> {|bytes_like bytes|} -> tkt:treekem_types bytes -> l:nat -> i:tree_index l -> pre:bytes_compatible_pre bytes -> x:treesync bytes tkt l i -> Lemma
-  ((ps_treesync tkt l i).is_valid pre x <==> treesync_has_pre pre x)
-let rec ps_treesync_is_valid #bytes #bl tkt l i pre x =
+val ps_treesync_is_well_formed: #bytes:Type0 -> {|bytes_like bytes|} -> tkt:treekem_types bytes -> l:nat -> i:tree_index l -> pre:bytes_compatible_pre bytes -> x:treesync bytes tkt l i -> Lemma
+  (is_well_formed_partial (ps_treesync tkt l i) pre x <==> treesync_has_pre pre x)
+let rec ps_treesync_is_well_formed #bytes #bl tkt l i pre x =
   match x with
   | TLeaf _ -> ()
   | TNode data left right ->
-    ps_treesync_is_valid tkt (l-1) (left_index i) pre left;
-    ps_treesync_is_valid tkt (l-1) (right_index i) pre right
+    ps_treesync_is_well_formed tkt (l-1) (left_index i) pre left;
+    ps_treesync_is_well_formed tkt (l-1) (right_index i) pre right
 
 val ps_as_tokens: #bytes:Type0 -> {|bytes_like bytes|} -> #as_token:Type0 -> parser_serializer bytes as_token -> l:nat -> i:tree_index l -> parser_serializer bytes (as_tokens bytes as_token l i)
 let ps_as_tokens #bytes #bl #as_token ps_token l i =
