fstar/MLS.TreeSync.NetworkTypes.fst
@@ -66,7 +66,7 @@ type leaf_node_source_nt =
 
 %splice [ps_leaf_node_source_nt] (gen_parser (`leaf_node_source_nt))
 %splice [ps_leaf_node_source_nt_length] (gen_length_lemma (`leaf_node_source_nt))
-%splice [ps_leaf_node_source_nt_is_valid] (gen_is_valid_lemma (`leaf_node_source_nt))
+%splice [ps_leaf_node_source_nt_is_well_formed] (gen_is_well_formed_lemma (`leaf_node_source_nt))
 
 /// struct {
 ///     ProtocolVersion versions<V>;
@@ -159,7 +159,7 @@ type leaf_node_data_nt (bytes:Type0) {|bytes_like bytes|} (tkt:treekem_types byt
 
 %splice [ps_leaf_node_data_nt] (gen_parser (`leaf_node_data_nt))
 %splice [ps_leaf_node_data_nt_length] (gen_length_lemma (`leaf_node_data_nt))
-%splice [ps_leaf_node_data_nt_is_valid] (gen_is_valid_lemma (`leaf_node_data_nt))
+%splice [ps_leaf_node_data_nt_is_well_formed] (gen_is_well_formed_lemma (`leaf_node_data_nt))
 
 type leaf_node_nt (bytes:Type0) {|bytes_like bytes|} (tkt:treekem_types bytes) = {
   data: leaf_node_data_nt bytes tkt;
@@ -167,7 +167,7 @@ type leaf_node_nt (bytes:Type0) {|bytes_like bytes|} (tkt:treekem_types bytes) =
 }
 
 %splice [ps_leaf_node_nt] (gen_parser (`leaf_node_nt))
-%splice [ps_leaf_node_nt_is_valid] (gen_is_valid_lemma (`leaf_node_nt))
+%splice [ps_leaf_node_nt_is_well_formed] (gen_is_well_formed_lemma (`leaf_node_nt))
 
 instance parseable_serializeable_leaf_node_nt (bytes:Type0) {|bytes_like bytes|} (tkt:treekem_types bytes): parseable_serializeable bytes (leaf_node_nt bytes tkt) = mk_parseable_serializeable (ps_leaf_node_nt tkt)
 
@@ -240,7 +240,7 @@ type leaf_node_tbs_nt (bytes:Type0) {|bytes_like bytes|} (tkt:treekem_types byte
 
 %splice [ps_leaf_node_tbs_nt] (gen_parser (`leaf_node_tbs_nt))
 %splice [ps_leaf_node_tbs_nt_length] (gen_length_lemma (`leaf_node_tbs_nt))
-%splice [ps_leaf_node_tbs_nt_is_valid] (gen_is_valid_lemma (`leaf_node_tbs_nt))
+%splice [ps_leaf_node_tbs_nt_is_well_formed] (gen_is_well_formed_lemma (`leaf_node_tbs_nt))
 
 instance parseable_serializeable_leaf_node_tbs_nt (bytes:Type0) {|bytes_like bytes|} (tkt:treekem_types bytes): parseable_serializeable bytes (leaf_node_tbs_nt bytes tkt) = mk_parseable_serializeable (ps_leaf_node_tbs_nt tkt)
 
@@ -298,7 +298,7 @@ type parent_node_nt (bytes:Type0) {|bytes_like bytes|} (tkt:treekem_types bytes)
 }
 
 %splice [ps_parent_node_nt] (gen_parser (`parent_node_nt))
-%splice [ps_parent_node_nt_is_valid] (gen_is_valid_lemma (`parent_node_nt))
+%splice [ps_parent_node_nt_is_well_formed] (gen_is_well_formed_lemma (`parent_node_nt))
 
 instance parseable_serializeable_parent_node_nt (bytes:Type0) {|bytes_like bytes|} (tkt:treekem_types bytes): parseable_serializeable bytes (parent_node_nt bytes tkt) = mk_parseable_serializeable (ps_parent_node_nt tkt)
 
@@ -315,7 +315,7 @@ type node_type_nt =
 
 %splice [ps_node_type_nt] (gen_parser (`node_type_nt))
 %splice [ps_node_type_nt_length] (gen_length_lemma (`node_type_nt))
-%splice [ps_node_type_nt_is_valid] (gen_is_valid_lemma (`node_type_nt))
+%splice [ps_node_type_nt_is_well_formed] (gen_is_well_formed_lemma (`node_type_nt))
 
 /// struct {
 ///     NodeType node_type;
